Prove CLAM/goal44

benchmarks/CLAM/goal44.v
@@ -1,8 +1,10 @@
-Require Import Nat Arith.
+Require Import Nat Arith Bool.
 
-Inductive Nat : Type := succ : Nat -> Nat |  zero : Nat.
+Inductive Nat : Type := zero : Nat | succ : Nat -> Nat.
 
-Inductive Lst : Type := cons : Nat -> Lst -> Lst |  nil : Lst.
+Scheme Equality for Nat.
+
+Inductive Lst : Type := nil : Lst | cons : Nat -> Lst -> Lst.
 
 Inductive Tree : Type := node : Nat -> Tree -> Tree -> Tree |  leaf : Tree.
 
@@ -12,13 +14,10 @@ with ZLst : Type := zcons : Pair -> ZLst -> ZLst |  znil : ZLst.
 Fixpoint mem (mem_arg0 : Nat) (mem_arg1 : Lst) : bool
            := match mem_arg0, mem_arg1 with
               | x, nil => false
-              | x, cons y z => orb (eqb x y) (mem x z)
+              | x, cons y z => orb (Nat_beq x y) (mem x z)
               end.
 
-Fixpoint lst_mem (lst_mem_arg0 : Nat) (lst_mem_arg1 : Lst) : bool
-           := match lst_mem_arg0, lst_mem_arg1 with
-              | n, x => mem n x
-              end.
+Definition lst_mem := mem.
 
 Fixpoint lst_intersection (lst_intersection_arg0 : Lst) (lst_intersection_arg1 : Lst) : Lst
            := match lst_intersection_arg0, lst_intersection_arg1 with
@@ -26,7 +25,30 @@ Fixpoint lst_intersection (lst_intersection_arg0 : Lst) (lst_intersection_arg1 :
               | cons n x, y => if lst_mem n y then cons n (lst_intersection x y) else lst_intersection x y
               end.
 
+Lemma Nat_beq_eq : forall (x y : Nat), Nat_beq x y = true -> x = y.
+Proof.
+  intros.
+  generalize dependent y.
+  induction x.
+  - intros. destruct y.
+    + reflexivity.
+    + discriminate.
+  - intros. destruct y.
+    + discriminate.
+    + simpl in H. apply IHx in H. rewrite H. reflexivity.
+Qed.
+
 Theorem theorem0 : forall (x : Nat) (y : Lst) (z : Lst), and (eq (lst_mem x y) true) (eq (lst_mem x z) true) -> eq (lst_mem x (lst_intersection y z)) true.
 Proof.
-Admitted.
-
+  intros.
+  destruct H.
+  induction y.
+  - discriminate.
+  - simpl in H. apply orb_prop in H. destruct H.
+    + simpl. destruct (lst_mem n z) eqn:?.
+      * simpl. rewrite H. reflexivity.
+      * rewrite (Nat_beq_eq x n H) in H0. rewrite H0 in Heqb. discriminate.
+    + apply IHy in H. simpl. destruct (lst_mem n z) eqn:?.
+      * simpl. rewrite H. apply orb_true_r.
+      * assumption.
+Qed.
